backend/LinearC.v
@@ -163,14 +163,15 @@ Definition current_locset (stk: stackframe): locset :=
 .
 
 (* Definition dummy_stacksize: Z := (admit "dummy_stacksize"). *)
-Definition dummy_code (sig: signature): code := [Lcall sig (admit "dummy_reg")].
-Definition dummy_function (sig: signature) := (mkfunction (admit "dummy_sig") 0 (dummy_code sig)).
+(* Definition dummy_code (sig: signature): code := [Lcall sig (admit "dummy_reg")]. *)
+Definition dummy_function (sig: signature) := (mkfunction sig 0 []).
 
 Definition dummy_stack (sig: signature) (ls: locset) :=
   Stackframe (dummy_function sig)
-              (Vptr (admit "dummy_fptr") Ptrofs.zero true)
-              ls
-              [] (* one may replace it with another another_dummy_code,
+              (* (Vptr (admit "dummy_fptr") Ptrofs.zero true) *)
+             Vundef
+             ls
+             [] (* one may replace it with another another_dummy_code,
 but then corresponding MachM's part should be transl_code another_dummy_code ... *)
 .
 Hint Unfold dummy_stack.
@@ -352,6 +353,7 @@ Section MODSEM.
   .
   Next Obligation.
     inv INIT0; inv INIT1; ss. clarify.
+    inv LOADARG. inv LOADARG0.
     determ_tac extcall_arguments_determ.
     rewrite RSPPTR in *. clarify.
   Qed.
